Garden/Plonky3/M.v
@@ -56,6 +56,13 @@ Module Array.
     {|
       get index := f (x.(get) index)
     |}.
+
+  Module Eq.
+    Definition t {A : Set} {N : Z} (x y : t A N) : Prop :=
+      forall (i : Z), 0 <= i < N -> x.(get) i = y.(get) i.
+
+    Axiom dec : forall {A : Set} {N : Z} (x y : Array.t A N), {t x y} + {~ t x y}.
+  End Eq.
 End Array.
 
 Module UnOp.
@@ -160,7 +167,7 @@ Module M.
   Definition for_each {A : Set} {N : Z} (f : A -> t unit) (x : Array.t A N) : t unit :=
     for_in_zero_to_n N (fun i => f (Array.get x i)).
 
-  (* helper: acting on all elements in an array, but returning a sum *)    
+  (* helper: acting on all elements in an array, but returning a sum *)
 
   Fixpoint sum_for_in_zero_to_n_aux {p} `{Prime p} (N : nat) (f : Z -> Z) : Z :=
     match N with
@@ -496,3 +503,161 @@ Proof.
   { rewrite <- (Z.mod_unique x p (-1) (p + x)) in *; lia. }
   { rewrite <- (Z.mod_unique x p 0 x) in *; lia. }
 Qed.
+
+(* TODO: prove with Coqtail *)
+Lemma sub_zero_equiv {p} `{Prime p} (x y : Z) :
+  BinOp.sub x y = 0 <->
+  UnOp.from x = UnOp.from y.
+Proof.
+Admitted.
+
+Lemma sum_for_in_zero_to_n_zeros_eq {p} `{Prime p} (N : Z) (f : Z -> Z)
+    (H_body : forall (i : Z), 0 <= i < N -> f i = 0) :
+  M.sum_for_in_zero_to_n N f = 0.
+Proof.
+Admitted.
+
+(** Rewrite rules for field operations. *)
+Module FieldRewrite.
+  Lemma from_zero {p} `{Prime p} : UnOp.from 0 = 0.
+  Proof.
+    reflexivity.
+  Qed.
+  Global Hint Rewrite @from_zero : field_rewrite.
+
+  Lemma from_one {p} `{Prime p} : UnOp.from 1 = 1.
+  Proof.
+  Admitted.
+  Global Hint Rewrite @from_one : field_rewrite.
+
+  Lemma from_from {p} `{Prime p} (x : Z) :
+    UnOp.from (UnOp.from x) = UnOp.from x.
+  Proof.
+    show_equality_modulo.
+  Qed.
+  Global Hint Rewrite @from_from : field_rewrite.
+
+  Lemma from_add {p} `{Prime p} (x y : Z) :
+    UnOp.from (BinOp.add x y) = BinOp.add x y.
+  Proof.
+    show_equality_modulo.
+  Qed.
+  Global Hint Rewrite @from_add : field_rewrite.
+
+  Lemma add_from_left {p} `{Prime p} (x y : Z) :
+    BinOp.add (UnOp.from x) y = BinOp.add x y.
+  Proof.
+    show_equality_modulo.
+  Qed.
+  Global Hint Rewrite @add_from_left : field_rewrite.
+
+  Lemma add_from_right {p} `{Prime p} (x y : Z) :
+    BinOp.add x (UnOp.from y) = BinOp.add x y.
+  Proof.
+    show_equality_modulo.
+  Qed.
+  Global Hint Rewrite @add_from_right : field_rewrite.
+
+  Lemma sub_from_left {p} `{Prime p} (x y : Z) :
+    BinOp.sub (UnOp.from x) y = BinOp.sub x y.
+  Proof.
+    show_equality_modulo.
+  Qed.
+  Global Hint Rewrite @sub_from_left : field_rewrite.
+
+  Lemma sub_from_right {p} `{Prime p} (x y : Z) :
+    BinOp.sub x (UnOp.from y) = BinOp.sub x y.
+  Proof.
+    show_equality_modulo.
+  Qed.
+  Global Hint Rewrite @sub_from_right : field_rewrite.
+
+  Lemma mul_from_left {p} `{Prime p} (x y : Z) :
+    BinOp.mul (UnOp.from x) y = BinOp.mul x y.
+  Proof.
+    show_equality_modulo.
+  Qed.
+  Global Hint Rewrite @mul_from_left : field_rewrite.
+
+  Lemma mul_from_right {p} `{Prime p} (x y : Z) :
+    BinOp.mul x (UnOp.from y) = BinOp.mul x y.
+  Proof.
+    show_equality_modulo.
+  Qed.
+  Global Hint Rewrite @mul_from_right : field_rewrite.
+
+  Lemma from_sub {p} `{Prime p} (x y : Z) :
+    UnOp.from (BinOp.sub x y) = BinOp.sub x y.
+  Proof.
+    show_equality_modulo.
+  Qed.
+  Global Hint Rewrite @from_sub : field_rewrite.
+
+  Lemma from_mul {p} `{Prime p} (x y : Z) :
+    UnOp.from (BinOp.mul x y) = BinOp.mul x y.
+  Proof.
+    show_equality_modulo.
+  Qed.
+  Global Hint Rewrite @from_mul : field_rewrite.
+
+  Lemma add_zero_left {p} `{Prime p} (x : Z) :
+    BinOp.add 0 x = UnOp.from x.
+  Proof.
+    show_equality_modulo.
+  Qed.
+  Global Hint Rewrite @add_zero_left : field_rewrite.
+
+  Lemma add_zero_right {p} `{Prime p} (x : Z) :
+    BinOp.add x 0 = UnOp.from x.
+  Proof.
+    show_equality_modulo.
+    f_equal; lia.
+  Qed.
+  Global Hint Rewrite @add_zero_right : field_rewrite.
+
+  Lemma sub_zero_left {p} `{Prime p} (x : Z) :
+    BinOp.sub 0 x = UnOp.from (-x).
+  Proof.
+    show_equality_modulo.
+  Qed.
+  Global Hint Rewrite @sub_zero_left : field_rewrite.
+
+  Lemma sub_zero_right {p} `{Prime p} (x : Z) :
+    BinOp.sub x 0 = UnOp.from x.
+  Proof.
+    show_equality_modulo.
+    f_equal; lia.
+  Qed.
+  Global Hint Rewrite @sub_zero_right : field_rewrite.
+
+  Lemma mul_zero_left {p} `{Prime p} (x : Z) :
+    BinOp.mul 0 x = 0.
+  Proof.
+    show_equality_modulo.
+  Qed.
+  Global Hint Rewrite @mul_zero_left : field_rewrite.
+
+  Lemma mul_zero_right {p} `{Prime p} (x : Z) :
+    BinOp.mul x 0 = 0.
+  Proof.
+    show_equality_modulo.
+    now replace (x * 0) with 0 by lia.
+  Qed.
+  Global Hint Rewrite @mul_zero_right : field_rewrite.
+
+  Lemma mul_one_left {p} `{Prime p} (x : Z) :
+    BinOp.mul 1 x = UnOp.from x.
+  Proof.
+    show_equality_modulo.
+    now replace (1 * x) with x by lia.
+  Qed.
+  Global Hint Rewrite @mul_one_left : field_rewrite.
+
+  Lemma mul_one_right {p} `{Prime p} (x : Z) :
+    BinOp.mul x 1 = UnOp.from x.
+  Proof.
+    show_equality_modulo.
+    now replace (x * 1) with x by lia.
+  Qed.
+  Global Hint Rewrite @mul_one_right : field_rewrite.
+End FieldRewrite.
